Update UTF8 Encode, Decode to be methods, not return Result<>

src/extern/dotnet/UTF8.cs
@@ -6,28 +6,16 @@ using charseq = Dafny.Sequence<char>;
 
 namespace UTF8 {
   public partial class __default {
-    public static STL.Result<byteseq> Encode(Dafny.Sequence<char> str) {
+    public static byteseq Encode(Dafny.Sequence<char> str) {
       UTF8Encoding utf8 = new UTF8Encoding(false, true);
-      try {
-          byte[] utf8Bytes = utf8.GetBytes(str.Elements);
-          return new STL.Result_Success<byteseq>(byteseq.FromArray(utf8Bytes));
-      } catch(EncoderFallbackException e) {
-          return new STL.Result_Failure<byteseq>(charseq.FromArray("Input contains invalid Unicode characters".ToCharArray()));
-      } catch(ArgumentNullException e) {
-          return new STL.Result_Failure<byteseq>(charseq.FromArray("Input is null".ToCharArray()));
-      }
+      byte[] utf8Bytes = utf8.GetBytes(str.Elements);
+      return byteseq.FromArray(utf8Bytes);
     }
 
-    public static STL.Result<Dafny.Sequence<char>> Decode(byteseq bytes) {
+    public static Dafny.Sequence<char> Decode(byteseq bytes) {
       UTF8Encoding utf8 = new UTF8Encoding(false, true);
-      try {
-          string decoded = utf8.GetString(bytes.Elements);
-          return new STL.Result_Success<Dafny.Sequence<char>>(charseq.FromArray(decoded.ToCharArray()));
-      } catch(ArgumentException e) {
-          // GetString is defined as returning ArgumentException, ArgumentNullException, DecoderFallbackException
-          // Both ArgumentNullException and DecoderFallbackException are children of ArgumentException
-          return new STL.Result_Failure<Dafny.Sequence<char>>(charseq.FromArray("Input contains an invalid Unicode code point".ToCharArray()));
-      }
+      string decoded = utf8.GetString(bytes.Elements);
+      return charseq.FromArray(decoded.ToCharArray());
     }
   }
 }
