src/SDK/MessageBody.dfy
@@ -24,8 +24,19 @@ module MessageBody {
   import EncryptionSuites
   import UTF8
 
-  const BODY_AAD_CONTENT_REGULAR_FRAME := UTF8.Encode("AWSKMSEncryptionClient Frame").value
-  const BODY_AAD_CONTENT_FINAL_FRAME := UTF8.Encode("AWSKMSEncryptionClient Final Frame").value
+  const AWS_KMS_ENCRYPTION_CLIENT_REGULAR_FRAME := "AWSKMSEncryptionClient Frame";
+  method GetBodyAADContentRegularFrame() returns (res: UTF8.ValidUTF8Bytes)
+  {
+    var encoded := UTF8.Encode(AWS_KMS_ENCRYPTION_CLIENT_REGULAR_FRAME);
+    return encoded;
+  }
+
+  const AWS_KMS_ENCRYPTION_CLIENT_FINAL_FRAME := "AWSKMSEncryptionClient Final Frame";
+  method GetBodyAADContentFinalFrame() returns (res: UTF8.ValidUTF8Bytes)
+  {
+    var encoded := UTF8.Encode(AWS_KMS_ENCRYPTION_CLIENT_FINAL_FRAME);
+    return encoded;
+  }
 
   const START_SEQUENCE_NUMBER: uint32 := 1
   const ENDFRAME_SEQUENCE_NUMBER: uint32 := 0xFFFF_FFFF
@@ -168,7 +179,9 @@ module MessageBody {
   }
 
   method BodyAAD(messageID: seq<uint8>, final: bool, sequenceNumber: uint32, length: uint64) returns (aad: seq<uint8>) {
-    var contentAAD := if final then BODY_AAD_CONTENT_FINAL_FRAME else BODY_AAD_CONTENT_REGULAR_FRAME;
+    var bodyAADFinalFrame := GetBodyAADContentFinalFrame();
+    var bodyAADRegularFrame := GetBodyAADContentRegularFrame();
+    var contentAAD := if final then bodyAADFinalFrame else bodyAADRegularFrame;
     aad := messageID + contentAAD + UInt32ToSeq(sequenceNumber) + UInt64ToSeq(length);
   }
 
